reorganized aggregation definitions

systems/AggregationAux.v
@@ -599,6 +599,96 @@ rewrite /sum_fold.
 by case H_find: (NMap.find _ _) => [m0|]; first by aac_reflexivity.
 Qed.
 
+Lemma nodup_notin : 
+  forall (A : Type) (a : A) (l l' : list A),
+    NoDup (l ++ a :: l') ->
+    ~ In a (l ++ l').
+Proof.
+move => A a.
+elim => /=; first by move => l' H_nd; inversion H_nd; subst.
+move => a' l IH l' H_nd.
+inversion H_nd; subst.
+move => H_in.
+case: H_in => H_in.
+  case: H1.
+  apply in_or_app.
+  by right; left.
+contradict H_in.
+exact: IH.
+Qed.
+
+Lemma permutation_split : 
+  forall (A : Type) (ns ns' : list A) (n : A),
+  Permutation (n :: ns) ns' ->
+  exists ns0, exists ns1, ns' = ns0 ++ n :: ns1.
+Proof.
+move => A ns ns' n H_pm.
+have H_in: In n (n :: ns) by left. 
+have H_in': In n ns'.
+  move: H_pm H_in. 
+  exact: Permutation_in.
+by apply In_split in H_in'.
+Qed.
+
+Lemma nodup_app_split_right : 
+  forall (A : Type) (ns0 ns1 : list A), 
+    NoDup (ns0 ++ ns1) -> NoDup ns1.
+Proof.
+move => A.
+elim => [|n ns0 IH] ns1 H_nd //.
+inversion H_nd => {l H0 x H}.
+exact: IH.
+Qed.
+
+Lemma nodup_in_not_in_right : 
+  forall (A : Type) (ns0 ns1 : list A) (x : A),
+    NoDup (ns0 ++ ns1) -> In x ns0 -> ~ In x ns1.
+Proof.
+move => A.
+elim => //=.
+move => n ns0 IH ns1 x H_nd H_in.
+inversion H_nd => {l H0 x0 H}.
+case: H_in => H_in; last exact: IH.
+rewrite H_in in H1.
+move => H_in'.
+case: H1.
+apply in_or_app.
+by right.
+Qed.
+
+Lemma nodup_in_not_in_left : 
+  forall (A : Type) (ns0 ns1 : list A) (x : A),
+    NoDup (ns0 ++ ns1) -> In x ns1 -> ~ In x ns0.
+Proof.
+move => A.
+elim => [|n ns0 IH] ns1 x H_nd H_in //.
+inversion H_nd => {l H0 x0 H}.
+move => H_in'.
+case: H_in' => H_in'.
+  rewrite H_in' in H1.
+  case: H1.
+  apply in_or_app.
+  by right.
+contradict H_in'.
+exact: (IH _ _ H2).
+Qed.
+
+Lemma nodup_app_split_left : 
+  forall (A : Type) (ns0 ns1 : list A), 
+    NoDup (ns0 ++ ns1) -> NoDup ns0.
+Proof.
+move => A.
+elim => [|n ns0 IH] ns1 H_nd; first exact: NoDup_nil.
+inversion H_nd => {l H0 x H}.
+apply NoDup_cons.
+  move => H_in.
+  case: H1.
+  apply in_or_app.
+  by left.
+move: H2.
+exact: IH.
+Qed.
+
 Class AggregationData (A :  Type) :=
   {
     local : A -> m ;
@@ -649,6 +739,103 @@ rewrite IH; first by gsimpl; aac_reflexivity.
 move => d' H_in.
 apply: H_cn.
 by right.
+Qed.
+
+Definition Nodes_data (ns : list name) (state : name -> A) : list A :=
+fold_right (fun (n : name) (l' : list A) => n.(state) :: l') [] ns.
+
+Lemma sum_local_split :
+  forall ns0 ns1 state n,
+    sum_local (Nodes_data (ns0 ++ n :: ns1) state) =
+    n.(state).(local) * sum_local (Nodes_data (ns0 ++ ns1) state).
+Proof.
+elim => /=; first by move => ns1 state n; aac_reflexivity.
+move => n ns IH ns1 state n'.
+rewrite IH /=.
+by gsimpl.
+Qed.
+
+Lemma sum_aggregate_split :
+  forall ns0 ns1 state n,
+    sum_aggregate (Nodes_data (ns0 ++ n :: ns1) state) =
+    n.(state).(aggregate) * sum_aggregate (Nodes_data (ns0 ++ ns1) state).
+Proof.
+elim => /=; first by move => ns1 state n; aac_reflexivity.
+move => n ns IH ns1 state n'.
+rewrite IH /=.
+by gsimpl.
+Qed.
+
+Lemma Nodes_data_not_in : 
+forall n' d state ns,
+~ In n' ns ->
+fold_right
+  (fun (n : name) (l : list A) =>
+     (match name_eq_dec n n' with
+      | left _ => d 
+      | right _ => n.(state) 
+      end) :: l) [] ns = Nodes_data ns state.
+Proof.
+move => n' d state.
+elim => //.
+move => a l IH H_in.
+rewrite /=.
+case name_eq_dec => H_dec; first by case: H_in; left.
+rewrite IH => //.
+move => H_in'.
+by case: H_in; right.
+Qed.
+
+Lemma Nodes_data_split :
+  forall ns0 ns1 state,
+    Nodes_data (ns0 ++ ns1) state =
+    Nodes_data ns0 state ++ Nodes_data ns1 state.
+Proof.
+elim => //.
+move => n ns0 IH ns1 state.
+rewrite /=.
+by rewrite IH.
+Qed.
+
+Lemma sum_sent_distr : 
+  forall dl dl',
+    sum_sent (dl ++ dl') = sum_sent dl * sum_sent dl'.
+Proof.
+elim => /=; first by move => dl'; gsimpl.
+move => d dl IH dl'.
+rewrite IH.
+by aac_reflexivity.
+Qed.
+
+Lemma sum_received_distr : 
+  forall dl dl',
+    sum_received (dl ++ dl') = sum_received dl * sum_received dl'.
+Proof.
+elim => /=; first by move => dl'; gsimpl.
+move => d dl IH dl'.
+rewrite IH.
+by aac_reflexivity.
+Qed.
+
+Lemma sum_sent_Nodes_data_distr : 
+  forall ns0 ns1 state,
+    sum_sent (Nodes_data ns0 state) * sum_sent (Nodes_data ns1 state) =
+    sum_sent (Nodes_data (ns0 ++ ns1) state).
+Proof.
+elim => [|n ns0 IH] ns1 net /=; first by gsimpl.
+rewrite -IH.
+by aac_reflexivity.
+Qed.
+
+Lemma sum_received_Nodes_data_distr : 
+  forall ns0 ns1 state,
+    (sum_received (Nodes_data ns1 state))^-1 * (sum_received (Nodes_data ns0 state))^-1 = 
+    (sum_received (Nodes_data (ns0 ++ ns1) state))^-1.
+Proof.
+elim => [|n ns0 IH] ns1 state /=; first by gsimpl.
+gsimpl.
+rewrite -IH.
+by aac_reflexivity.
 Qed.
 
 End AggregationProps.
